Added nicer synax for UNREST

theories/models/utp_cml/examples/Dwarf.thy
@@ -1,46 +1,80 @@
+(******************************************************************************)
+(* Project: CML model for Isabelle/UTP                                        *)
+(* File: Dwarf.thy                                                            *)
+(* Author: Simon Foster, University of York (UK)                              *)
+(******************************************************************************)
+
+header {* CML Dwarf Signal Example *}
+
+(*<*)
 theory Dwarf
 imports 
   "../utp_cml"
 begin
+(*>*)
 
-ML {*
-  structure dwarf_simps =
-    Named_Thms (val name = @{binding dwarf_simps} val description = "dwarf simps")
-*}
+subsubsection {* Dwarf Signal Types *}
 
-setup dwarf_simps.setup
+text {* A \emph{Dwarf Signal} is a kind of railway signal which is
+used at the side of track when space is limited. An illustration is
+shown in Figure \ref{fig:dwarfsignal}. It has three lamps which are
+displayed in different configurations to give instructions to train
+drivers. The signal's three lamps are named L1--L3, as illustrated,
+and different configurations of a signal can be written using set
+notation, for instance this signal is in $\{L1, L2\}$ which means
+\textbf{Stop}. We begin by setting up three abbreviations to represent
+these three strings. *}
 
 abbreviation "L1 \<equiv> ''L1''"
 abbreviation "L2 \<equiv> ''L2''"
 abbreviation "L3 \<equiv> ''L3''"
 
-text {* First set of VDM types, which depend on nothing else *}
+text {* Next we start to construct the basic types for the Dwarf
+signal, including the \texttt{LampId}, an enumeration of the three
+signal states, and \texttt{Signal} which a (finite) set of
+\texttt{LampId}s.*}
 
 abbreviation "LampId   \<equiv> \<parallel><L1> | <L2> | <L3>\<parallel>"
 abbreviation "Signal   \<equiv> \<parallel>@set of @LampId\<parallel>"
 
-text {* Next define the "proper states" for the signal *}
+text {* The signal has a total of four \emph{proper states} which are
+the well-defined commands a signal can convey to a driver. When all
+lamps are off (indicated by the empty set $\{\}$) the signal is in the
+\textbf{Dark} state, which is a power saving mode for when the signal
+is not in use. The three remaining proper states \textbf{Stop},
+\textbf{Warning} and \textbf{Drive} are indicated by a combination of
+two lamps and correspond to the positions of an old-style semaphore
+signal. We define these possible values below: *}
 
 definition "dark     \<equiv> +|{}|+"
 definition "stop     \<equiv> +|{<L1>, <L2>}|+"
 definition "warning  \<equiv> +|{<L1>, <L3>}|+"
 definition "drive    \<equiv> +|{<L2>, <L3>}|+"
 
+text {* We also add the definitional equations for these values to the
+evaluation tactics, so that proofs can be performed about them: *}
+
 declare dark_def [eval,evalp]
 declare stop_def [eval,evalp]
 declare warning_def [eval,evalp]
 declare drive_def [eval,evalp]
 
-text {* A proper state is a signal which falls within this set *}
+text {* Next we set up the datatype for proper states. It consists of
+a signal which is in one of the four states: \textbf{Dark},
+\textbf{Stop}, \textbf{Warning} and \textbf{Drive}, specified through
+an invariant. *}
 
 abbreviation 
-  "ProperState \<equiv> \<parallel>@Signal inv ps == (^ps^ in @set {&dark, &stop, &warning, &drive})\<parallel>"
+  "ProperState \<equiv> 
+     \<parallel>@Signal inv ps == (^ps^ in @set {&dark, &stop, &warning, &drive})\<parallel>"
 
-text {* Setting up a record type is currently a little complicated, though could
-        easily be automatically generated. First we create a new unit type to act
-        as the "tag" for this record so that it can be distinguished from others. We
-        create an instance of the tag class which proves its a unit type and associates
-        a string with it (the name of the type). *}
+text {* Next we create a datatype to represent the state of the entire
+Dwarf Signal, which we specify as a CML record. Setting up a record
+type is currently a little complicated, though the CML tool
+automatically generates them. First we create a new unit type to act
+as the "tag" for this record so that it can be distinguished from
+others. We create an instance of the tag class which proves its a unit
+type and associates a string with it (the name of the type). *}
 
 typedef DwarfType_Tag = "{True}" by auto
 instantiation DwarfType_Tag :: tag
@@ -51,39 +85,51 @@ instance
 end
 
 text {* Next we create a collection of fields associated with the tag, and give each
-        the position in record and its VDM type. *}
+        the position in record and its CML type. *}
 
-abbreviation "lastproperstate_fld    \<equiv> MkField TYPE(DwarfType_Tag) #1 \<parallel>@ProperState\<parallel>"
-abbreviation "desiredproperstate_fld \<equiv> MkField TYPE(DwarfType_Tag) #2 \<parallel>@ProperState\<parallel>"
-abbreviation "turnoff_fld            \<equiv> MkField TYPE(DwarfType_Tag) #3 \<parallel>@set of @LampId\<parallel>"
-abbreviation "turnon_fld             \<equiv> MkField TYPE(DwarfType_Tag) #4 \<parallel>@set of @LampId\<parallel>"
-abbreviation "laststate_fld          \<equiv> MkField TYPE(DwarfType_Tag) #5 \<parallel>@Signal\<parallel>"
-abbreviation "currentstate_fld       \<equiv> MkField TYPE(DwarfType_Tag) #6 \<parallel>@Signal\<parallel>"
+abbreviation "lastproperstate_fld \<equiv> 
+  MkField TYPE(DwarfType_Tag) #1 \<parallel>@ProperState\<parallel>"
+
+abbreviation "desiredproperstate_fld \<equiv> 
+  MkField TYPE(DwarfType_Tag) #2 \<parallel>@ProperState\<parallel>"
+
+abbreviation "turnoff_fld \<equiv> 
+  MkField TYPE(DwarfType_Tag) #3 \<parallel>@set of @LampId\<parallel>"
+
+abbreviation "turnon_fld \<equiv> 
+  MkField TYPE(DwarfType_Tag) #4 \<parallel>@set of @LampId\<parallel>"
+
+abbreviation "laststate_fld \<equiv> 
+  MkField TYPE(DwarfType_Tag) #5 \<parallel>@Signal\<parallel>"
+
+abbreviation "currentstate_fld \<equiv> 
+  MkField TYPE(DwarfType_Tag) #6 \<parallel>@Signal\<parallel>"
 
 text {* Then we use these fields to create selector functions for the record, which
-        can be used directly in UTP/VDM predicates *}
+        can be used directly in UTP/CML predicates *}
 
-abbreviation "lastproperstate    \<equiv> SelectRec lastproperstate_fld"
+abbreviation "lastproperstate \<equiv> SelectRec lastproperstate_fld"
 abbreviation "desiredproperstate \<equiv> SelectRec desiredproperstate_fld"
-abbreviation "turnoff            \<equiv> SelectRec turnoff_fld"
-abbreviation "turnon             \<equiv> SelectRec turnon_fld"
-abbreviation "laststate          \<equiv> SelectRec laststate_fld"
-abbreviation "currentstate       \<equiv> SelectRec currentstate_fld"
+abbreviation "turnoff \<equiv> SelectRec turnoff_fld"
+abbreviation "turnon \<equiv> SelectRec turnon_fld"
+abbreviation "laststate \<equiv> SelectRec laststate_fld"
+abbreviation "currentstate \<equiv> SelectRec currentstate_fld"
 
 text {* Finally we create the actual type by giving the list of fields and the associated
-        invariant. We also create a record constructor, mk_DwarfType. *}
+        invariant. We also create a record constructor, \texttt{mk\_DwarfType}. *}
 
 definition 
-  "DwarfType \<equiv> \<parallel>[ lastproperstate_fld
-                , desiredproperstate_fld
-                , turnoff_fld
-                , turnon_fld
-                , laststate_fld
-                , currentstate_fld] 
-                inv d == ((^d^.currentstate setminus ^d^.turnoff) union ^d^.turnon 
-                            = ^d^.desiredproperstate)
-                         and 
-                         (^d^.turnon inter ^d^.turnoff = {})\<parallel>"
+  "DwarfType \<equiv> 
+     \<parallel>[ lastproperstate_fld
+      , desiredproperstate_fld
+      , turnoff_fld
+      , turnon_fld
+      , laststate_fld
+      , currentstate_fld] 
+     inv d == ((^d^.currentstate setminus ^d^.turnoff) union ^d^.turnon 
+               = ^d^.desiredproperstate)
+              and 
+              (^d^.turnon inter ^d^.turnoff = {})\<parallel>"
 
 declare DwarfType_def [eval,evalp]
 
@@ -91,13 +137,20 @@ definition "mk_DwarfType \<equiv> MkRec DwarfType"
 
 declare mk_DwarfType_def [eval,evalp]
 
+(*<*)
 lemma mkd: "|mk_DwarfType(&stop, &stop, {}, {}, &stop, &stop) hasType @DwarfType| = |true|"
   by (cml_tac)
+(*>*)
+ 
+subsubsection {* Safety Properties *}
 
-text {* Safety Properties *}
+text {* We specify the safety properties of the Dwarf signal. These
+are specified by use of CML functions from the Dwarf Signal type to a
+boolean. *}
 
 definition 
-  "NeverShowAll = |lambda d @ ^d^.#1.currentstate <> {<L1>,<L2>,<L3>}|"
+  "NeverShowAll = 
+    |lambda d @ ^d^.#1.currentstate <> {<L1>,<L2>,<L3>}|"
 
 declare NeverShowAll_def [eval,evalp]
 
@@ -111,19 +164,22 @@ declare MaxOneLampChange_def [eval,evalp]
 
 definition
   "ForbidStopToDrive = 
-     |lambda d @ (^d^.#1.lastproperstate = &stop) => ^d^.#1.desiredproperstate <> &drive|"
+     |lambda d @ (^d^.#1.lastproperstate = &stop) 
+               => ^d^.#1.desiredproperstate <> &drive|"
   
 declare ForbidStopToDrive_def [eval,evalp]
 
 definition
   "DarkOnlyToStop = 
-     |lambda d @ (^d^.#1.lastproperstate = &dark) => ^d^.#1.desiredproperstate in @set {&dark,&stop}|" 
+     |lambda d @ (^d^.#1.lastproperstate = &dark) 
+               => ^d^.#1.desiredproperstate in @set {&dark,&stop}|" 
   
 declare DarkOnlyToStop_def [eval,evalp]
 
 definition
   "DarkOnlyFromStop = 
-     |lambda d @ (^d^.#1.desiredproperstate = &dark) => ^d^.#1.lastproperstate in @set {&dark,&stop}|"
+     |lambda d @ (^d^.#1.desiredproperstate = &dark) 
+               => ^d^.#1.lastproperstate in @set {&dark,&stop}|"
 
 declare DarkOnlyFromStop_def [eval,evalp]
 
@@ -136,28 +192,39 @@ definition
 
 declare DwarfSignal_def [eval,evalp]
 
-lemma "|NeverShowAll(mk_DwarfType(&stop, &stop, {}, {}, &stop, &stop))| = |true|"
+text {* To exemplify CML proof goals, we show that an initialised
+state of the signal satisfies the safety invariants. *}
+
+lemma NeverShowAll_Init:
+  "|NeverShowAll(mk_DwarfType(&stop, &stop, {}, {}, &stop, &stop))| = |true|"
   by (cml_tac)
 
-lemma "|MaxOneLampChange(mk_DwarfType(&stop, &stop, {}, {}, &stop, &stop))| = |true|"
+lemma MaxOneLampChange_Init:
+  "|MaxOneLampChange(mk_DwarfType(&stop, &stop, {}, {}, &stop, &stop))| = |true|"
   by (cml_tac)
 
-lemma "|ForbidStopToDrive(mk_DwarfType(&stop, &stop, {}, {}, &stop, &stop))| = |true|"
+lemma ForbidStopToDrive_Init:
+  "|ForbidStopToDrive(mk_DwarfType(&stop, &stop, {}, {}, &stop, &stop))| = |true|"
   by (cml_tac)
 
-lemma "|DarkOnlyToStop(mk_DwarfType(&stop, &stop, {}, {}, &stop, &stop))| = |true|"
+lemma DarkOnlyToStop_Init:
+  "|DarkOnlyToStop(mk_DwarfType(&stop, &stop, {}, {}, &stop, &stop))| = |true|"
   by (cml_tac)
 
-lemma "|DarkOnlyFromStop(mk_DwarfType(&stop, &stop, {}, {}, &stop, &stop))| = |true|"
+lemma DarkOnlyFromStop_Init:
+  "|DarkOnlyFromStop(mk_DwarfType(&stop, &stop, {}, {}, &stop, &stop))| = |true|"
   by (cml_tac)
 
+(*<*)
 lemma sdty: "|mk_DwarfType(&stop, &stop, {}, {}, &stop, &stop) hasType @DwarfSignal| = |true|"
   by (cml_tac)
+(*>*)
 
-text {* The Dwarf Signal has a single state variable which gives 
-        the state of the signal. *}
+subsubsection {* Reactive Behaviour *}
 
-text {* Channels *}
+text {* We first define the channels with to specify the interaction
+of the Dwarf signal. Channels can carry data so they all take a CML
+type to specify this. *}
 
 definition "init = MkChanD ''init'' \<parallel>()\<parallel>"
 definition "light = MkChanD ''light'' \<parallel>@LampId\<parallel>"
@@ -165,19 +232,30 @@ definition "extinguish = MkChanD ''extinguish'' \<parallel>@LampId\<parallel>"
 definition "setPS = MkChanD ''setPS'' \<parallel>@ProperState\<parallel>"
 definition "shine = MkChanD ''shine'' \<parallel>@Signal\<parallel>"
 
+text {* The Dwarf Signal process defines a namespace to avoid clashes
+with state variables, operations and actions in other processes. We
+provide the namespace in Isabelle by way of an Isabelle locale. *}
+
 locale DwarfProcess
 begin
 
-text {* State *}
+text {* The Dwarf Signal has a single state variable which gives 
+        the state of the signal. *}
 
 abbreviation "dw \<equiv> MkVarD ''dw'' DwarfType"
 
-definition "DwarfInv \<equiv> `\<lparr> $dw hasType @DwarfType \<rparr> \<turnstile> \<lparr> $dw\<acute> hasType @DwarfType \<rparr>`"
+text {* We also specify the invariant of the Dwarf Signal as a UTP
+design. *}
 
-text {* Operations *}
+definition "DwarfInv \<equiv> 
+  `\<lparr> $dw hasType @DwarfType \<rparr> \<turnstile> \<lparr> $dw\<acute> hasType @DwarfType \<rparr>`"
 
-definition "Init = `true \<turnstile> (dw := mk_DwarfType(&stop, &stop, {}, {}, &stop, &stop))`"
+text {* Next we specify the operations for the Dwarf Signal process. *}
 
+definition "Init = 
+  `true \<turnstile> (dw := mk_DwarfType(&stop, &stop, {}, {}, &stop, &stop))`"
+
+(*<*)
 lemma UNREST_vexpr_empty [unrest]: 
   "UNREST_PEXPR vs vexpr_empty"
   by (simp add:UNREST_PEXPR_def vexpr_empty_def evalp)
@@ -215,10 +293,12 @@ lemma "DwarfInv \<sqsubseteq> Init"
   apply (rule unrest)
   apply (rule unrest)
 oops
+(*>*)
 
 definition 
   "SetNewProperState st = 
-      `\<lparr>($dw).currentstate = ($dw).desiredproperstate and ^st^ <> ($dw).currentstate\<rparr> 
+      `\<lparr>($dw).currentstate = ($dw).desiredproperstate 
+        and ^st^ <> ($dw).currentstate\<rparr> 
        \<turnstile> dw := mk_DwarfType( ($dw).currentstate
                            , ($dw).currentstate setminus ^st^
                            , ^st^ setminus ($dw).currentstate
@@ -256,22 +336,22 @@ definition
        [] ((setPS?(s) -> SetNewProperState(&s)); DWARF)
        [] (shine!(($dw).currentstate) -> DWARF))`"
 
-(* Working test *)
+text {* Working test *}
 definition
   "TEST1 = `setPS!&warning -> extinguish!<L2> -> light!<L3> 
            -> setPS!&drive -> extinguish!<L1> -> light!<L2> -> STOP`"
 
-(* Tries to turn on 3 lights simulaneously *)
+text {* Tries to turn on 3 lights simulaneously *}
 definition
   "TEST2 = `setPS!&warning -> light!<L3> -> extinguish!<L2> 
            -> setPS!&drive -> extinguish!<L1> -> light!<L2> -> STOP`"
 
-(* Tries to go from dark to warning *)
+text {* Tries to go from dark to warning *}
 definition
   "TEST3 = `setPS!&dark -> extinguish!<L1> -> extinguish!<L2> -> setPS!&warning -> 
             light!<L1> -> light!<L2> -> STOP`"
 
-(* Tries to go from stop to drive *)
+text {* Tries to go from stop to drive *}
 definition
   "TEST4 = `setPS!&drive -> extinguish!<L1> -> light!<L3> -> STOP`"
 
@@ -280,6 +360,7 @@ definition "DWARF_TEST2 = `DWARF [|{setPS\<down>,light\<down>,extinguish\<down>}
 definition "DWARF_TEST3 = `DWARF [|{setPS\<down>,light\<down>,extinguish\<down>}|] TEST3`"
 definition "DWARF_TEST4 = `DWARF [|{setPS\<down>,light\<down>,extinguish\<down>}|] TEST4`"
 
+text {* The main action of the process. *}
 definition 
   "MainAction = DWARF"
 
